<?xml version='1.0' encoding='ISO-8859-1'?>
<!DOCTYPE rdf:RDF [
	 <!ENTITY rdf  'http://www.w3.org/1999/02/22-rdf-syntax-ns#'>
	 <!ENTITY rdfs 'http://www.w3.org/TR/1999/PR-rdf-schema-19990303#'>
]>

<rdf:RDF
  xmlns:rdf="&rdf;"
  xmlns:rdfs="&rdfs;">


<rdfs:Class rdf:about="&rdf;Statement"
   rdfs:comment="A triple consisting of a  predicate, a subject, and an object." />


<rdfs:Class rdf:about="&rdf;Property"
   rdfs:comment="A name of a property, defining specific meaning for the property" />


<rdf:Property rdf:about="&rdf;predicate"
   rdfs:comment="Identifies the property used in a statement when representing the statement in reified form">
  <rdfs:domain rdf:resource="&rdf;Statement" />
  <rdfs:range rdf:resource="&rdf;Property" />
  <rdfs:range rdf:resource="&rdfs;Literal"/>
</rdf:Property>


<rdf:Property rdf:about="&rdf;subject"
   rdfs:comment="Identifies the resource that a statement is describing when representing the statement in reified form">
  <rdfs:domain rdf:resource="&rdf;Statement" />
</rdf:Property>


<rdf:Property rdf:about="&rdf;object"
   rdfs:comment="Identifies the object of a statement when representing the statement in reified form">
  <rdfs:domain rdf:resource="&rdf;Statement" />
  <rdfs:range rdf:resource="&rdfs;Literal"/>
  <rdfs:range rdf:resource="&rdfs;Resource"/>
</rdf:Property>




<rdf:Property rdf:about="&rdf;type"
   rdfs:comment="Identifies the Class of a resource" />


<rdf:Property rdf:about="&rdf;value"
   rdfs:comment="Identifies the principal value (usually a string) of a property when the property value is a structured resource" />


</rdf:RDF>
